The Section \ref{s_1_1} defined the \textbf{product rule}. It can be written in two forms:
\begin{center}
    $P(a \wedge b) = P(a|b)P(b)$ and $P(a \wedge b) = P(b|a)P(a)$
\end{center}
Combining the right-hand side of each equation and dividing by $P(a)$, we get the \textbf{Bayes' rule}.
\begin{definition}[title={Bayes' theorem}]
    \begin{center}
        $P(b|a) = \frac{P(a|b)P(b)}{P(a)}$ 
    \end{center} \vspace{3.5pt}
    or in distribution form:
    \begin{center}
        $\mathbf{P}(Y|X) = \frac{\mathbf{P}(X|Y)\mathbf{P}(Y)}{\mathbf{P}(X)}$ 
    \end{center}
\end{definition}
This turns out to be very useful for assessing \textbf{diagnostic} probability from \textbf{causal} probability.